Completely new definition of sequence/function limits. (Add the IR_inf definition to make the limit definitions compatible)

limits.v
@@ -1,10 +1,13 @@
-Require Import CauchySeq.
 Require Import ZArith.
 Require Import Classical_Prop.
+
+Require Import SAMPL.sequences.
 
 (**
 * Definitions
 *)
+
+Section Limit_definitions.
 
 (**
 ** Limits of real functions
@@ -16,20 +19,18 @@ Variable f : CSetoid_un_op IR.
 We define the limit [l] of the function [f x] as [x] approaches [x0] with 
 9 different cases (depending on [l] and [x0]) :
 - [x0] is finite :
-  - [l] is finite :
-  - [l] is +&infin; :
-  - [l] is -&infin; :
-- [x0] is +&infin; :
-  - [l] is finite :
-  - [l] is +&infin; :
-  - [l] is -&infin; :
-- [x0] is -&infin; :
-  - [l] is finite :
-  - [l] is +&infin; :
-  - [l] is -&infin; :
+  - [l] is finite : $$x_0 \in \mathbb{R}, \lim\limits_{x \to x_0} f(x) = l \in \mathbb{R}$$
+  - [l] is $$+\infty$$ : $$x_0 \in \mathbb{R}, \lim\limits_{x \to x_0} f(x) = +\infty$$
+  - [l] is $$-\infty$$ : $$x_0 \in \mathbb{R}, \lim\limits_{x \to x_0} f(x) = -\infty$$
+- [x0] is $$+\infty$$ :
+  - [l] is finite : $$\lim\limits_{x \to +\infty} f(x) = l \in \mathbb{R}$$
+  - [l] is $$+\infty$$ : $$\lim\limits_{x \to +\infty} f(x) = +\infty$$
+  - [l] is $$-\infty$$ : $$\lim\limits_{x \to +\infty} f(x) = -\infty$$
+- [x0] is $$-\infty$$ :
+  - [l] is finite : $$\lim\limits_{x \to -\infty} f(x) = l \in \mathbb{R}$$
+  - [l] is $$+\infty$$ : $$\lim\limits_{x \to -\infty} f(x) = +\infty$$
+  - [l] is $$-\infty$$ : $$\lim\limits_{x \to -\infty} f(x) = -\infty$$
 *)
-
-Require Import RealFuncts.
 
 Inductive limit : Type :=
     | xFinite_lFinite : IR->IR->limit
@@ -44,6 +45,18 @@ Inductive limit : Type :=
 
 (**
 We assign a predicate to each limit :
+- [x0] is finite :
+  - [l] is finite : $$\forall \epsilon>0, \exists \delta>0, \forall x \in \[x_0 - \delta, x_0 + \delta\] \cap I, |f(x)-l| \leq \epsilon$$
+  - [l] is $$+\infty$$ : $$\forall A \in \mathbb{R}, \exists \delta>0, \forall x \in \[x_0 - \delta, x_0 + \delta\] \cap I, f(x) \geq A$$
+  - [l] is $$-\infty$$ : $$\forall A \in \mathbb{R}, \exists \delta>0, \forall x \in \[x_0 - \delta, x_0 + \delta\] \cap I, f(x) \leq A$$
+- [x0] is $$+\infty$$ :
+  - [l] is finite : $$\forall \epsilon>0, \exists a \in \mathbb{R}, \forall x \in I, x \geq a \Rightarrow |f(x)-l| \leq \epsilon$$
+  - [l] is $$+\infty$$ : $$\forall A \in \mathbb{R}, \exists a \in \mathbb{R}, \forall x \in I, x \geq a \Rightarrow f(x) \geq A$$
+  - [l] is $$-\infty$$ : $$\forall A \in \mathbb{R}, \exists a \in \mathbb{R}, \forall x \in I, x \geq a \Rightarrow f(x) \leq A$$
+- [x0] is $$-\infty$$ :
+  - [l] is finite : $$\forall \epsilon>0, \exists a \in \mathbb{R}, \forall x \in I, x \leq a \Rightarrow |f(x)-l| \leq \epsilon$$
+  - [l] is $$+\infty$$ : $$\forall A \in \mathbb{R}, \exists a \in \mathbb{R}, \forall x \in I, x \leq a \Rightarrow f(x) \geq A$$
+  - [l] is $$-\infty$$ : $$\forall A \in \mathbb{R}, \exists a \in \mathbb{R}, \forall x \in I, x \leq a \Rightarrow f(x) \leq A$$
 *)
 
 Definition limitProp (L : limit) : CProp :=
@@ -70,6 +83,37 @@ Definition limitProp (L : limit) : CProp :=
     end.
 
 (**
+In the previous definitions, $$x_0 \in \overline{\mathbb{R}}$$ and $$l \in \overline{\mathbb{R}}$$, so we
+define to helper definitions to deal with them as [IR_inf] :
+*)
+
+Definition limit_variable (L : limit) : IR_inf :=
+    match L with
+        | xFinite_lFinite x0 _ => real x0
+        | xFinite_lPlusInf x0 => real x0
+        | xFinite_lMinusInf x0 => real x0
+        | xPlusInf_lFinite _ => pInf
+        | xPlusInf_lPlusInf => pInf
+        | xPlusInf_lMinusInf => pInf
+        | xMinusInf_lFinite _ => mInf
+        | xMinusInf_lPlusInf => mInf
+        | xMinusInf_lMinusInf => mInf
+    end.
+
+Definition limit_value (L : limit) : IR_inf :=
+    match L with
+        | xFinite_lFinite _ l => real l
+        | xFinite_lPlusInf _ => pInf
+        | xFinite_lMinusInf _ => mInf
+        | xPlusInf_lFinite l => real l
+        | xPlusInf_lPlusInf => pInf
+        | xPlusInf_lMinusInf => mInf
+        | xMinusInf_lFinite l => real l
+        | xMinusInf_lPlusInf => pInf
+        | xMinusInf_lMinusInf => mInf
+    end.
+
+(**
 * Theorems
 *)
 
@@ -77,6 +121,16 @@ Definition limitProp (L : limit) : CProp :=
 Sequential characterization of a limit
 *)
 
+End Limit_definitions.
+
+Hypothesis x0 : IR_inf.
+Hypothesis l : IR_inf.
+Hypothesis f : CSetoid_un_op IR.
+
+Theorem sequential_limit : (forall (L : limit), limitProp f L -> limit_variable L = x0 -> limit_value L = l)
+    <-> (forall (Un : nat->IR), forall (L fL : Un_limit), Un_limitProp Un L -> Un_limitProp (fun n => f (Un n)) fL 
+        -> Un_limit_value L = x0 -> Un_limit_value fL = l).
+Admitted.
 
 (**
 * Applications
@@ -101,12 +155,12 @@ Definition periodic_function (T : IR) : Prop :=
 Definition constant_function : Prop :=
     forall (x y : IR), f x = f y.
 
-Theorem app1 : forall (T : IR), periodic_function T -> 
+(*Theorem app1 : forall (T : IR), periodic_function T -> 
     forall (l : IR), limitProp (xPlusInf_lFinite l) -> constant_function.
     intros. unfold constant_function. intros. apply NNPP ; intro. unfold periodic_function in H. destruct H.
     assert (f x = f (x[+]zring x0[*]T)) by apply H.
     assert (f y = f (y[+]zring x0[*]T)) by apply H.
-Admitted.
+Admitted.*)
 
 (** 
 ** Appli 2 : Prove that a function has no limit
@@ -115,7 +169,7 @@ Admitted.
 (**
 1) sin(x)
 We extract the 
-*) 
+*)
 
 
 
