reals.v
@@ -1,0 +1,27 @@
+Require Export CoRN.reals.CauchySeq.
+
+(**
+* Definitions
+*)
+
+(**
+We define a helper type for the limits : 
+$$\overline{\mathbb{R}} = \mathbb{R} \cup \{+\infty\} \cup \{-\infty\}$$
+*)
+
+Inductive IR_inf : Type :=
+    | real : IR -> IR_inf
+    | pInf : IR_inf
+    | mInf : IR_inf.
+
+(**
+** Absolute value
+*)
+
+(**
+We use the CoRN definition, located in CoRN.algebra.COrdAbs.
+*)
+
+(** 
+$$|a - b| \leq e \equiv$$ [AbsSmall e (a - b)] $$\equiv$$ [AbsSmall e (b - a)]
+*)
